\documentclass{article}
\usepackage{proof}
\usepackage{amssymb,amsmath}
\usepackage{relsize}
\usepackage[
    % a0paper,
    % landscape,
    papersize={100in,20in},
    margin={2in,2in}
    %total={1800in, 10in},
    ]{geometry}


\def\code#1{\texttt{#1}}

\title{Big Proof Trees}
\author{Iain Moncrief}
\date{February 2023}

\begin{document}
\relscale{0.1}

\maketitle

\section{Introduction}


$$\infer[]{\{\ \},[] \vdash \code{fib 5}  \Rightarrow \code{5}}{\infer[]{\{\ \},[] \vdash \code{fib}  \Rightarrow \code{(closure n -> if (n < 2) then n else (fib ((n - 1)) + fib ((n - 2))))}}{\{\ \},[] \vdash \code{(fun n -> if (n < 2) then n else (fib ((n - 1)) + fib ((n - 2))))}  \Rightarrow \code{(closure n -> if (n < 2) then n else (fib ((n - 1)) + fib ((n - 2))))}} && \{\ \},[] \vdash \code{5}  \Rightarrow \code{5} && \infer[]{\{\ \},[\code{n}  \mapsto \code{5}] \vdash \code{if (n < 2) then n else (fib ((n - 1)) + fib ((n - 2)))}  \Rightarrow \code{5}}{\infer[]{\{\ \},[\code{n}  \mapsto \code{5}] \vdash \code{(n < 2)}  \Rightarrow \code{False}}{\{\ \},[\code{n}  \mapsto \code{5}] \vdash \code{n}  \Rightarrow \code{5} && \{\ \},[] \vdash \code{2}  \Rightarrow \code{2}} && \infer[]{\{\ \},[\code{n}  \mapsto \code{5}] \vdash \code{(fib ((n - 1)) + fib ((n - 2)))}  \Rightarrow \code{5}}{\infer[]{\{\ \},[\code{n}  \mapsto \code{5}] \vdash \code{fib ((n - 1))}  \Rightarrow \code{3}}{\infer[]{\{\ \},[] \vdash \code{fib}  \Rightarrow \code{(closure n -> if (n < 2) then n else (fib ((n - 1)) + fib ((n - 2))))}}{\{\ \},[] \vdash \code{(fun n -> if (n < 2) then n else (fib ((n - 1)) + fib ((n - 2))))}  \Rightarrow \code{(closure n -> if (n < 2) then n else (fib ((n - 1)) + fib ((n - 2))))}} && \infer[]{\{\ \},[\code{n}  \mapsto \code{5}] \vdash \code{(n - 1)}  \Rightarrow \code{4}}{\{\ \},[\code{n}  \mapsto \code{5}] \vdash \code{n}  \Rightarrow \code{5} && \{\ \},[] \vdash \code{1}  \Rightarrow \code{1}} && \infer[]{\{\ \},[\code{n}  \mapsto \code{4}] \vdash \code{if (n < 2) then n else (fib ((n - 1)) + fib ((n - 2)))}  \Rightarrow \code{3}}{\infer[]{\{\ \},[\code{n}  \mapsto \code{4}] \vdash \code{(n < 2)}  \Rightarrow \code{False}}{\{\ \},[\code{n}  \mapsto \code{4}] \vdash \code{n}  \Rightarrow \code{4} && \{\ \},[] \vdash \code{2}  \Rightarrow \code{2}} && \infer[]{\{\ \},[\code{n}  \mapsto \code{4}] \vdash \code{(fib ((n - 1)) + fib ((n - 2)))}  \Rightarrow \code{3}}{\infer[]{\{\ \},[\code{n}  \mapsto \code{4}] \vdash \code{fib ((n - 1))}  \Rightarrow \code{2}}{\infer[]{\{\ \},[] \vdash \code{fib}  \Rightarrow \code{(closure n -> if (n < 2) then n else (fib ((n - 1)) + fib ((n - 2))))}}{\{\ \},[] \vdash \code{(fun n -> if (n < 2) then n else (fib ((n - 1)) + fib ((n - 2))))}  \Rightarrow \code{(closure n -> if (n < 2) then n else (fib ((n - 1)) + fib ((n - 2))))}} && \infer[]{\{\ \},[\code{n}  \mapsto \code{4}] \vdash \code{(n - 1)}  \Rightarrow \code{3}}{\{\ \},[\code{n}  \mapsto \code{4}] \vdash \code{n}  \Rightarrow \code{4} && \{\ \},[] \vdash \code{1}  \Rightarrow \code{1}} && \infer[]{\{\ \},[\code{n}  \mapsto \code{3}] \vdash \code{if (n < 2) then n else (fib ((n - 1)) + fib ((n - 2)))}  \Rightarrow \code{2}}{\infer[]{\{\ \},[\code{n}  \mapsto \code{3}] \vdash \code{(n < 2)}  \Rightarrow \code{False}}{\{\ \},[\code{n}  \mapsto \code{3}] \vdash \code{n}  \Rightarrow \code{3} && \{\ \},[] \vdash \code{2}  \Rightarrow \code{2}} && \infer[]{\{\ \},[\code{n}  \mapsto \code{3}] \vdash \code{(fib ((n - 1)) + fib ((n - 2)))}  \Rightarrow \code{2}}{\infer[]{\{\ \},[\code{n}  \mapsto \code{3}] \vdash \code{fib ((n - 1))}  \Rightarrow \code{1}}{\infer[]{\{\ \},[] \vdash \code{fib}  \Rightarrow \code{(closure n -> if (n < 2) then n else (fib ((n - 1)) + fib ((n - 2))))}}{\{\ \},[] \vdash \code{(fun n -> if (n < 2) then n else (fib ((n - 1)) + fib ((n - 2))))}  \Rightarrow \code{(closure n -> if (n < 2) then n else (fib ((n - 1)) + fib ((n - 2))))}} && \infer[]{\{\ \},[\code{n}  \mapsto \code{3}] \vdash \code{(n - 1)}  \Rightarrow \code{2}}{\{\ \},[\code{n}  \mapsto \code{3}] \vdash \code{n}  \Rightarrow \code{3} && \{\ \},[] \vdash \code{1}  \Rightarrow \code{1}} && \infer[]{\{\ \},[\code{n}  \mapsto \code{2}] \vdash \code{if (n < 2) then n else (fib ((n - 1)) + fib ((n - 2)))}  \Rightarrow \code{1}}{\infer[]{\{\ \},[\code{n}  \mapsto \code{2}] \vdash \code{(n < 2)}  \Rightarrow \code{False}}{\{\ \},[\code{n}  \mapsto \code{2}] \vdash \code{n}  \Rightarrow \code{2} && \{\ \},[] \vdash \code{2}  \Rightarrow \code{2}} && \infer[]{\{\ \},[\code{n}  \mapsto \code{2}] \vdash \code{(fib ((n - 1)) + fib ((n - 2)))}  \Rightarrow \code{1}}{\infer[]{\{\ \},[\code{n}  \mapsto \code{2}] \vdash \code{fib ((n - 1))}  \Rightarrow \code{1}}{\infer[]{\{\ \},[] \vdash \code{fib}  \Rightarrow \code{(closure n -> if (n < 2) then n else (fib ((n - 1)) + fib ((n - 2))))}}{\{\ \},[] \vdash \code{(fun n -> if (n < 2) then n else (fib ((n - 1)) + fib ((n - 2))))}  \Rightarrow \code{(closure n -> if (n < 2) then n else (fib ((n - 1)) + fib ((n - 2))))}} && \infer[]{\{\ \},[\code{n}  \mapsto \code{2}] \vdash \code{(n - 1)}  \Rightarrow \code{1}}{\{\ \},[\code{n}  \mapsto \code{2}] \vdash \code{n}  \Rightarrow \code{2} && \{\ \},[] \vdash \code{1}  \Rightarrow \code{1}} && \infer[]{\{\ \},[\code{n}  \mapsto \code{1}] \vdash \code{if (n < 2) then n else (fib ((n - 1)) + fib ((n - 2)))}  \Rightarrow \code{1}}{\infer[]{\{\ \},[\code{n}  \mapsto \code{1}] \vdash \code{(n < 2)}  \Rightarrow \code{True}}{\{\ \},[\code{n}  \mapsto \code{1}] \vdash \code{n}  \Rightarrow \code{1} && \{\ \},[] \vdash \code{2}  \Rightarrow \code{2}} && \{\ \},[\code{n}  \mapsto \code{1}] \vdash \code{n}  \Rightarrow \code{1}}} && \infer[]{\{\ \},[\code{n}  \mapsto \code{2}] \vdash \code{fib ((n - 2))}  \Rightarrow \code{0}}{\infer[]{\{\ \},[] \vdash \code{fib}  \Rightarrow \code{(closure n -> if (n < 2) then n else (fib ((n - 1)) + fib ((n - 2))))}}{\{\ \},[] \vdash \code{(fun n -> if (n < 2) then n else (fib ((n - 1)) + fib ((n - 2))))}  \Rightarrow \code{(closure n -> if (n < 2) then n else (fib ((n - 1)) + fib ((n - 2))))}} && \infer[]{\{\ \},[\code{n}  \mapsto \code{2}] \vdash \code{(n - 2)}  \Rightarrow \code{0}}{\{\ \},[\code{n}  \mapsto \code{2}] \vdash \code{n}  \Rightarrow \code{2} && \{\ \},[] \vdash \code{2}  \Rightarrow \code{2}} && \infer[]{\{\ \},[\code{n}  \mapsto \code{0}] \vdash \code{if (n < 2) then n else (fib ((n - 1)) + fib ((n - 2)))}  \Rightarrow \code{0}}{\infer[]{\{\ \},[\code{n}  \mapsto \code{0}] \vdash \code{(n < 2)}  \Rightarrow \code{True}}{\{\ \},[\code{n}  \mapsto \code{0}] \vdash \code{n}  \Rightarrow \code{0} && \{\ \},[] \vdash \code{2}  \Rightarrow \code{2}} && \{\ \},[\code{n}  \mapsto \code{0}] \vdash \code{n}  \Rightarrow \code{0}}}}}} && \infer[]{\{\ \},[\code{n}  \mapsto \code{3}] \vdash \code{fib ((n - 2))}  \Rightarrow \code{1}}{\infer[]{\{\ \},[] \vdash \code{fib}  \Rightarrow \code{(closure n -> if (n < 2) then n else (fib ((n - 1)) + fib ((n - 2))))}}{\{\ \},[] \vdash \code{(fun n -> if (n < 2) then n else (fib ((n - 1)) + fib ((n - 2))))}  \Rightarrow \code{(closure n -> if (n < 2) then n else (fib ((n - 1)) + fib ((n - 2))))}} && \infer[]{\{\ \},[\code{n}  \mapsto \code{3}] \vdash \code{(n - 2)}  \Rightarrow \code{1}}{\{\ \},[\code{n}  \mapsto \code{3}] \vdash \code{n}  \Rightarrow \code{3} && \{\ \},[] \vdash \code{2}  \Rightarrow \code{2}} && \infer[]{\{\ \},[\code{n}  \mapsto \code{1}] \vdash \code{if (n < 2) then n else (fib ((n - 1)) + fib ((n - 2)))}  \Rightarrow \code{1}}{\infer[]{\{\ \},[\code{n}  \mapsto \code{1}] \vdash \code{(n < 2)}  \Rightarrow \code{True}}{\{\ \},[\code{n}  \mapsto \code{1}] \vdash \code{n}  \Rightarrow \code{1} && \{\ \},[] \vdash \code{2}  \Rightarrow \code{2}} && \{\ \},[\code{n}  \mapsto \code{1}] \vdash \code{n}  \Rightarrow \code{1}}}}}} && \infer[]{\{\ \},[\code{n}  \mapsto \code{4}] \vdash \code{fib ((n - 2))}  \Rightarrow \code{1}}{\infer[]{\{\ \},[] \vdash \code{fib}  \Rightarrow \code{(closure n -> if (n < 2) then n else (fib ((n - 1)) + fib ((n - 2))))}}{\{\ \},[] \vdash \code{(fun n -> if (n < 2) then n else (fib ((n - 1)) + fib ((n - 2))))}  \Rightarrow \code{(closure n -> if (n < 2) then n else (fib ((n - 1)) + fib ((n - 2))))}} && \infer[]{\{\ \},[\code{n}  \mapsto \code{4}] \vdash \code{(n - 2)}  \Rightarrow \code{2}}{\{\ \},[\code{n}  \mapsto \code{4}] \vdash \code{n}  \Rightarrow \code{4} && \{\ \},[] \vdash \code{2}  \Rightarrow \code{2}} && \infer[]{\{\ \},[\code{n}  \mapsto \code{2}] \vdash \code{if (n < 2) then n else (fib ((n - 1)) + fib ((n - 2)))}  \Rightarrow \code{1}}{\infer[]{\{\ \},[\code{n}  \mapsto \code{2}] \vdash \code{(n < 2)}  \Rightarrow \code{False}}{\{\ \},[\code{n}  \mapsto \code{2}] \vdash \code{n}  \Rightarrow \code{2} && \{\ \},[] \vdash \code{2}  \Rightarrow \code{2}} && \infer[]{\{\ \},[\code{n}  \mapsto \code{2}] \vdash \code{(fib ((n - 1)) + fib ((n - 2)))}  \Rightarrow \code{1}}{\infer[]{\{\ \},[\code{n}  \mapsto \code{2}] \vdash \code{fib ((n - 1))}  \Rightarrow \code{1}}{\infer[]{\{\ \},[] \vdash \code{fib}  \Rightarrow \code{(closure n -> if (n < 2) then n else (fib ((n - 1)) + fib ((n - 2))))}}{\{\ \},[] \vdash \code{(fun n -> if (n < 2) then n else (fib ((n - 1)) + fib ((n - 2))))}  \Rightarrow \code{(closure n -> if (n < 2) then n else (fib ((n - 1)) + fib ((n - 2))))}} && \infer[]{\{\ \},[\code{n}  \mapsto \code{2}] \vdash \code{(n - 1)}  \Rightarrow \code{1}}{\{\ \},[\code{n}  \mapsto \code{2}] \vdash \code{n}  \Rightarrow \code{2} && \{\ \},[] \vdash \code{1}  \Rightarrow \code{1}} && \infer[]{\{\ \},[\code{n}  \mapsto \code{1}] \vdash \code{if (n < 2) then n else (fib ((n - 1)) + fib ((n - 2)))}  \Rightarrow \code{1}}{\infer[]{\{\ \},[\code{n}  \mapsto \code{1}] \vdash \code{(n < 2)}  \Rightarrow \code{True}}{\{\ \},[\code{n}  \mapsto \code{1}] \vdash \code{n}  \Rightarrow \code{1} && \{\ \},[] \vdash \code{2}  \Rightarrow \code{2}} && \{\ \},[\code{n}  \mapsto \code{1}] \vdash \code{n}  \Rightarrow \code{1}}} && \infer[]{\{\ \},[\code{n}  \mapsto \code{2}] \vdash \code{fib ((n - 2))}  \Rightarrow \code{0}}{\infer[]{\{\ \},[] \vdash \code{fib}  \Rightarrow \code{(closure n -> if (n < 2) then n else (fib ((n - 1)) + fib ((n - 2))))}}{\{\ \},[] \vdash \code{(fun n -> if (n < 2) then n else (fib ((n - 1)) + fib ((n - 2))))}  \Rightarrow \code{(closure n -> if (n < 2) then n else (fib ((n - 1)) + fib ((n - 2))))}} && \infer[]{\{\ \},[\code{n}  \mapsto \code{2}] \vdash \code{(n - 2)}  \Rightarrow \code{0}}{\{\ \},[\code{n}  \mapsto \code{2}] \vdash \code{n}  \Rightarrow \code{2} && \{\ \},[] \vdash \code{2}  \Rightarrow \code{2}} && \infer[]{\{\ \},[\code{n}  \mapsto \code{0}] \vdash \code{if (n < 2) then n else (fib ((n - 1)) + fib ((n - 2)))}  \Rightarrow \code{0}}{\infer[]{\{\ \},[\code{n}  \mapsto \code{0}] \vdash \code{(n < 2)}  \Rightarrow \code{True}}{\{\ \},[\code{n}  \mapsto \code{0}] \vdash \code{n}  \Rightarrow \code{0} && \{\ \},[] \vdash \code{2}  \Rightarrow \code{2}} && \{\ \},[\code{n}  \mapsto \code{0}] \vdash \code{n}  \Rightarrow \code{0}}}}}}}}} && \infer[]{\{\ \},[\code{n}  \mapsto \code{5}] \vdash \code{fib ((n - 2))}  \Rightarrow \code{2}}{\infer[]{\{\ \},[] \vdash \code{fib}  \Rightarrow \code{(closure n -> if (n < 2) then n else (fib ((n - 1)) + fib ((n - 2))))}}{\{\ \},[] \vdash \code{(fun n -> if (n < 2) then n else (fib ((n - 1)) + fib ((n - 2))))}  \Rightarrow \code{(closure n -> if (n < 2) then n else (fib ((n - 1)) + fib ((n - 2))))}} && \infer[]{\{\ \},[\code{n}  \mapsto \code{5}] \vdash \code{(n - 2)}  \Rightarrow \code{3}}{\{\ \},[\code{n}  \mapsto \code{5}] \vdash \code{n}  \Rightarrow \code{5} && \{\ \},[] \vdash \code{2}  \Rightarrow \code{2}} && \infer[]{\{\ \},[\code{n}  \mapsto \code{3}] \vdash \code{if (n < 2) then n else (fib ((n - 1)) + fib ((n - 2)))}  \Rightarrow \code{2}}{\infer[]{\{\ \},[\code{n}  \mapsto \code{3}] \vdash \code{(n < 2)}  \Rightarrow \code{False}}{\{\ \},[\code{n}  \mapsto \code{3}] \vdash \code{n}  \Rightarrow \code{3} && \{\ \},[] \vdash \code{2}  \Rightarrow \code{2}} && \infer[]{\{\ \},[\code{n}  \mapsto \code{3}] \vdash \code{(fib ((n - 1)) + fib ((n - 2)))}  \Rightarrow \code{2}}{\infer[]{\{\ \},[\code{n}  \mapsto \code{3}] \vdash \code{fib ((n - 1))}  \Rightarrow \code{1}}{\infer[]{\{\ \},[] \vdash \code{fib}  \Rightarrow \code{(closure n -> if (n < 2) then n else (fib ((n - 1)) + fib ((n - 2))))}}{\{\ \},[] \vdash \code{(fun n -> if (n < 2) then n else (fib ((n - 1)) + fib ((n - 2))))}  \Rightarrow \code{(closure n -> if (n < 2) then n else (fib ((n - 1)) + fib ((n - 2))))}} && \infer[]{\{\ \},[\code{n}  \mapsto \code{3}] \vdash \code{(n - 1)}  \Rightarrow \code{2}}{\{\ \},[\code{n}  \mapsto \code{3}] \vdash \code{n}  \Rightarrow \code{3} && \{\ \},[] \vdash \code{1}  \Rightarrow \code{1}} && \infer[]{\{\ \},[\code{n}  \mapsto \code{2}] \vdash \code{if (n < 2) then n else (fib ((n - 1)) + fib ((n - 2)))}  \Rightarrow \code{1}}{\infer[]{\{\ \},[\code{n}  \mapsto \code{2}] \vdash \code{(n < 2)}  \Rightarrow \code{False}}{\{\ \},[\code{n}  \mapsto \code{2}] \vdash \code{n}  \Rightarrow \code{2} && \{\ \},[] \vdash \code{2}  \Rightarrow \code{2}} && \infer[]{\{\ \},[\code{n}  \mapsto \code{2}] \vdash \code{(fib ((n - 1)) + fib ((n - 2)))}  \Rightarrow \code{1}}{\infer[]{\{\ \},[\code{n}  \mapsto \code{2}] \vdash \code{fib ((n - 1))}  \Rightarrow \code{1}}{\infer[]{\{\ \},[] \vdash \code{fib}  \Rightarrow \code{(closure n -> if (n < 2) then n else (fib ((n - 1)) + fib ((n - 2))))}}{\{\ \},[] \vdash \code{(fun n -> if (n < 2) then n else (fib ((n - 1)) + fib ((n - 2))))}  \Rightarrow \code{(closure n -> if (n < 2) then n else (fib ((n - 1)) + fib ((n - 2))))}} && \infer[]{\{\ \},[\code{n}  \mapsto \code{2}] \vdash \code{(n - 1)}  \Rightarrow \code{1}}{\{\ \},[\code{n}  \mapsto \code{2}] \vdash \code{n}  \Rightarrow \code{2} && \{\ \},[] \vdash \code{1}  \Rightarrow \code{1}} && \infer[]{\{\ \},[\code{n}  \mapsto \code{1}] \vdash \code{if (n < 2) then n else (fib ((n - 1)) + fib ((n - 2)))}  \Rightarrow \code{1}}{\infer[]{\{\ \},[\code{n}  \mapsto \code{1}] \vdash \code{(n < 2)}  \Rightarrow \code{True}}{\{\ \},[\code{n}  \mapsto \code{1}] \vdash \code{n}  \Rightarrow \code{1} && \{\ \},[] \vdash \code{2}  \Rightarrow \code{2}} && \{\ \},[\code{n}  \mapsto \code{1}] \vdash \code{n}  \Rightarrow \code{1}}} && \infer[]{\{\ \},[\code{n}  \mapsto \code{2}] \vdash \code{fib ((n - 2))}  \Rightarrow \code{0}}{\infer[]{\{\ \},[] \vdash \code{fib}  \Rightarrow \code{(closure n -> if (n < 2) then n else (fib ((n - 1)) + fib ((n - 2))))}}{\{\ \},[] \vdash \code{(fun n -> if (n < 2) then n else (fib ((n - 1)) + fib ((n - 2))))}  \Rightarrow \code{(closure n -> if (n < 2) then n else (fib ((n - 1)) + fib ((n - 2))))}} && \infer[]{\{\ \},[\code{n}  \mapsto \code{2}] \vdash \code{(n - 2)}  \Rightarrow \code{0}}{\{\ \},[\code{n}  \mapsto \code{2}] \vdash \code{n}  \Rightarrow \code{2} && \{\ \},[] \vdash \code{2}  \Rightarrow \code{2}} && \infer[]{\{\ \},[\code{n}  \mapsto \code{0}] \vdash \code{if (n < 2) then n else (fib ((n - 1)) + fib ((n - 2)))}  \Rightarrow \code{0}}{\infer[]{\{\ \},[\code{n}  \mapsto \code{0}] \vdash \code{(n < 2)}  \Rightarrow \code{True}}{\{\ \},[\code{n}  \mapsto \code{0}] \vdash \code{n}  \Rightarrow \code{0} && \{\ \},[] \vdash \code{2}  \Rightarrow \code{2}} && \{\ \},[\code{n}  \mapsto \code{0}] \vdash \code{n}  \Rightarrow \code{0}}}}}} && \infer[]{\{\ \},[\code{n}  \mapsto \code{3}] \vdash \code{fib ((n - 2))}  \Rightarrow \code{1}}{\infer[]{\{\ \},[] \vdash \code{fib}  \Rightarrow \code{(closure n -> if (n < 2) then n else (fib ((n - 1)) + fib ((n - 2))))}}{\{\ \},[] \vdash \code{(fun n -> if (n < 2) then n else (fib ((n - 1)) + fib ((n - 2))))}  \Rightarrow \code{(closure n -> if (n < 2) then n else (fib ((n - 1)) + fib ((n - 2))))}} && \infer[]{\{\ \},[\code{n}  \mapsto \code{3}] \vdash \code{(n - 2)}  \Rightarrow \code{1}}{\{\ \},[\code{n}  \mapsto \code{3}] \vdash \code{n}  \Rightarrow \code{3} && \{\ \},[] \vdash \code{2}  \Rightarrow \code{2}} && \infer[]{\{\ \},[\code{n}  \mapsto \code{1}] \vdash \code{if (n < 2) then n else (fib ((n - 1)) + fib ((n - 2)))}  \Rightarrow \code{1}}{\infer[]{\{\ \},[\code{n}  \mapsto \code{1}] \vdash \code{(n < 2)}  \Rightarrow \code{True}}{\{\ \},[\code{n}  \mapsto \code{1}] \vdash \code{n}  \Rightarrow \code{1} && \{\ \},[] \vdash \code{2}  \Rightarrow \code{2}} && \{\ \},[\code{n}  \mapsto \code{1}] \vdash \code{n}  \Rightarrow \code{1}}}}}}}}}$$
\end{document}