\documentclass{article}
\usepackage{amsmath,amssymb}
\usepackage{proof}
\usepackage{stmaryrd}
\usepackage[letterpaper,margin=1cm]{geometry}


\title{Specification and Rules for LANG}


\def\code#1{\texttt{#1}}
\def\codesf#1{\textsf{#1}}
\def\por{\ | \ }
\def\rt{\Rightarrow}
\def\binop{\ \text{\textbullet}\ }
\def\xj#1#2{\langle #1 \ | \ #2 \rangle}
\def\envj#1#2#3{D, #1 \vdash #2 \rt #3}
\def\noenvj#1#2{#1 \rt #2}
\def\xnf#1#2#3{D,#1 : #2 \rightsquigarrow #3}
\def\sem#1{\llbracket #1 \rrbracket}


\begin{document}

\maketitle
\section*{Syntax}

%\begin{gather*}
%v\in Name \qquad 	n\in \mathbb Z \qquad b \in \{\code{True},\code{False}\}\qquad \binop\in \{\code{+},\code{-},\code{*},\code{/},\code{\&\&},\code{||}\}
%\end{gather*}
%\begin{align*}
%lit \in \textsc{Literal} ::= \ & v \por n \por b\\\\
%pat \in \textsc{Pattern} ::=\ & \code{( cons $lit$ $pat$ )}\\
%						\por & \code{nil}\\
%						\por & lit\\\\
%list \in \textsc{List} ::= \ & \code{cons $e$ $list$}\\
%							\por & \code{nil}\\\\
%e\in \textsc{Expr} ::= \ & lit\\
%				\por & list\\
%				\por & e \binop e\\
%				\por & \code{\char`\\\ $v$ -> $e$}\\
%				\por & e \ e\\
%				\por & \code{let $v$ = $e$ in $e$}\\
%				\por & \code{letrec $v$ = $e$ in $e$ }\\
%				\por & \code{case $e$ of \char`\{ \ $($ $pat$ -> $e$ ; $)^*$ \char`\}}
%\end{align*}
%
%\section*{Example}
%\begin{align*}
%\code{letrec odds xs = case xs of \char`\{}&\ \  \code{nil -> [];}\\
%&\ \ \code{(cons x (cons y ys)) -> cons x (odds ys);}\\
%\code{kassia\char`\}}	& \code{ in odds [1,2,3]}
%\end{align*}



\begin{gather*}
v\in \textsc{Name} \qquad 	n\in \mathbb Z \qquad b \in \{\codesf{True},\codesf{False}\}\qquad c\in \{\codesf a, \codesf b,\ldots\}\qquad \binop\in \{\code{+},\code{-},\code{*},\code{/},\code{\&\&},\code{||},\code{++},\code{==},\code{>},\code{<},\code{>=},\code{<=}\}
\end{gather*}
\begin{align*}
%lit \in \textsc{Literal} ::= \ & v \por n \por b\\
str \in \textsc{String} ::= \code{"} \ c^* \ \code{"}\\\\
list(t) \in \textsc{List}(t) ::= \ & \codesf{[} \ t (\codesf{,} \ t)^* \ \codesf{]} \por \codesf{[ ]}\\\\
f \in \textsc{BuiltIn} ::= \ & \codesf{head} \por \codesf{tail}\\\\
pat \in \textsc{Pattern} ::=\ & b\qquad :(\\\\
e\in \textsc{Expr} ::= \ & v \por n \por b\\
				\por & \codesf{' $c$ '}\\
				\por & str\\
				\por & list(e)\\
				\por & e \binop e\\
				\por & \codesf{fun} \ v \ \code{->}\ e\\
				\por & e \ e\\
				\por & \codesf{let $v$ = $e$ in $e$}\\
				\por & \codesf{if $e$ then $e$ else $e$}\\
				\por & \codesf{case $e$ of \code{\char`\{} \ $($ $pat$ \code{->} $e$ \code; $)^*$ \code{\char`\}}}\\
				\por & f \ e_1 \ \ldots \ e_n \qquad \text{where $\textsf{arity}(f)=n$}\\\\
val \in \textsc{Value} ::= \ & n \por b \por c \por str \por list(val) \por  (\textsf{closure} \ v\to e,\rho)\\\\
\rho,\sigma \in \textsc{LocalEnv} \subseteq &\left(\textsc{Name}\times \textsc{Value}\right)^*\\\\
D \in \textsc{GlobalEnv} \subseteq &\left(\textsc{Name}\times \textsc{Expr}\right)^*\\\\
stm \in \textsc{Assign} ::= \ & \codesf{$v$ = $e$}\\\\
prog \in \textsc{Program} ::= \ & (stm \ \code{\char`\\n})^* \\\\
\end{align*}

%\section*{Example}
%\begin{align*}
%\code{letrec odds xs = case xs of \char`\{}&\ \  \code{nil -> [];}\\
%&\ \ \code{(cons x (cons y ys)) -> cons x (odds ys);}\\
%\code{kassia\char`\}}	& \code{ in odds [1,2,3]}
%\end{align*}
\pagebreak


\pagebreak
\section*{Denotational Semantics}


\section*{Operational Semantics}

$$
\textsc{EvalJ} ::= \textsc{GlobalEnv} \times \textsc{LocalEnv} \times \textsc{Expr} \times \textsc{Value}
$$
$$
\envj{\rho}{e}{v}\subseteq \textsc{EvalJ}
$$

\

\


\begin{figure*}[h]
$$
\infer[\textsc{Lit}]{
	D,\rho \vdash v \Rightarrow v
}{
}
$$

$$
\infer[\textsc{LocalVar}]{
	D,\rho \vdash x \Rightarrow v
}{
	(x,v) \in \rho
}
$$

$$
\infer[\textsc{GlobalVar}]{
	D,\rho \vdash x \Rightarrow v
}{
	(x,e) \in D
	&
	D,\{\} \vdash e \Rightarrow v
}
$$

$$
\infer[\textsc{Op}]{
	D,\rho \vdash e_1 \binop e_2 \Rightarrow v
}{
	D,\rho \vdash e_1 \Rightarrow v_1
	&
	D,\rho \vdash e_2 \Rightarrow v_2
	&
	\llbracket \binop\rrbracket(v_1,v_2) = v
}
$$

$$
\infer[\textsc{Abs}]{
	D,\rho \vdash \codesf{fun } x\code{ -> } e \Rightarrow (\codesf{closure}\ x\to e,\rho)
}{
}
$$

$$
\infer[\textsc{App}]{
	D,\rho \vdash e_1\ e_2 \Rightarrow v
}{
	D,\rho \vdash e_1 \Rightarrow (\codesf{closure}\ x\to e,\sigma)
	&
	D,\rho \vdash e_2 \Rightarrow v_2
	&
	D,\sigma[x\mapsto v_2] \vdash e \Rightarrow v
}
$$

$$
\infer[\textsc{Let}]{
	D,\rho \vdash \codesf{let}\ x=e_1\ \codesf{in}\ e_2 \Rightarrow v
}{
	D,\rho \vdash e_1 \Rightarrow v_1
	&
	D,\rho[x\mapsto v_1] \vdash e_2 \Rightarrow v
}
$$

$$
\infer[\textsc{BuiltIn}]{
	\envj{\rho}{f \ e_1 \ \ldots \ e_n}{v}
}{
	\envj{\rho}{e_i}{v_i}
	&
	\sem{f}(v_1,\ldots,v_n)=v
}
$$

$$
\infer[\textsc{ListNil}]{
	\envj{\rho}{\codesf{[ ]}}{\codesf{[ ]}}
}{}
\qquad
\infer[\textsc{List}]{
	\envj{\rho}{\codesf{[}e_1,\ldots,e_n\codesf ]}{\codesf [v_1,\ldots,v_n\codesf ]}
}{
	\envj{\rho}{e_i}{v_i}
}
$$

$$
\infer[\textsc{IfTrue}]{
	D,\rho \vdash \codesf{if}\ e_1\ \codesf{then}\ e_2\ \codesf{else}\ e_3 \Rightarrow v_1
}{
	D,\rho \vdash e_1 \Rightarrow \codesf{True}
	&
	D,\rho \vdash e_2 \Rightarrow v_1
}
\qquad
\infer[\textsc{IfFalse}]{
	D,\rho \vdash \codesf{if}\ e_1\ \codesf{then}\ e_2\ \codesf{else}\ e_3 \Rightarrow v_2
}{
	D,\rho \vdash e_1 \Rightarrow \codesf{False}
	&
	D,\rho \vdash e_3 \Rightarrow v_2
}
$$

\caption{Operational Semantics for LANG.}
\end{figure*}

%\begin{figure*}[h]
%\begin{align*}
%\sem{\code{+}}(a,b)&=a+b\\
%\sem{\code{*}}(a,b)&=a \cdot b\\
%&\vdots\\
%\sem{\code{++}}(l_1,l_2)&=l_1l_2\\
%\sem{\code{>}}(a,b)&=\ldots\\
%&\vdots
%\end{align*}
%\begin{align*}
%\sem{\codesf{head}}(x:xs)&=x\\
%\sem{\codesf{tail}}(x:xs)&=xs
%\end{align*}
%\end{figure*}





\pagebreak
\section*{Explanation Form}

$$
\textsc{NoEnvEvalJ} ::=\textsc{Expr}\times\textsc{Value}
$$
$$
\noenvj{e}{v}\subseteq \textsc{NoEnvEvalJ}
$$

$$
\Delta\in \textsc{XEvalJ} ::= \textsc{EvalJ}\times \textsc{NoEnvEvalJ}^*
$$
$$
\xj{\envj{\rho}{e}{v}}{\Delta}
$$

\

\

\begin{figure*}[h]
$$
\infer[\textsc{XLit}]{
    \langle D, \rho \vdash v \Rightarrow v \ | \ [\ ] \ \rangle
}{}
$$

$$
\infer[\textsc{XVar}]{
    \langle D, \rho \vdash x \Rightarrow v \ | \ [\  ]\  \rangle
}{}
$$

$$
\infer[\textsc{XBinOp}]{
    \langle D, \rho \vdash e_1 \binop e_2 \Rightarrow v \ | \ e_1' \binop e_2' \Rightarrow v \rangle
}{
    D, \rho \vdash e_1 \Rightarrow v_1
    &
    D, \rho \vdash e_2 \Rightarrow v_2
    &
    \llbracket \binop \rrbracket(v_1, v_2) = v
    &
    D, \rho : e_1 \rightsquigarrow e_1'
    &
    D, \rho : e_2 \rightsquigarrow e_2'
}
$$

$$
\infer[\textsc{XLetFun}]{
    \langle D, \rho \vdash \codesf{let } x = e_1 \codesf{ in } e_2 \Rightarrow v \ | \ e_2' \Rightarrow v \rangle
}{
    D, \rho \vdash e_1 \Rightarrow v_1
    &
    v_1 = (\textsf{closure } z \to e', \rho')
    &
    D, \rho[x \mapsto v_1] \vdash e_2 \Rightarrow v_2
    &
    D, \rho[x \mapsto v_1] : e_2 \rightsquigarrow e_2'
}
$$

$$
\infer[\textsc{XLet}]{
    \langle D, \rho \vdash \codesf{let } x = e_1 \codesf{ in } e_2 \Rightarrow v \ | \ e_1' \Rightarrow v_1, e_2' \Rightarrow v \rangle
}{
    D, \rho \vdash e_1 \Rightarrow v_1
    &
    D, \rho[x \mapsto v_1] \vdash e_2 \Rightarrow v
    &
    D, \rho[x \mapsto v_1] : e_2 \rightsquigarrow e_2'
    &
    D, \rho : e_1 \rightsquigarrow e_1'
}
$$

$$
\infer[\textsc{XApp}]{
	\langle D, \rho \vdash e_1 \ e_2 \Rightarrow v \ | \ e_1' \ v_2 \Rightarrow v, e_2' \Rightarrow v_2, \Delta\rangle
}{
	D, \rho  \vdash e_1 \Rightarrow (\codesf{closure} \ x \to e,\sigma )
	&
	\xj{D, \rho \vdash e_2 \Rightarrow v_2}{\Delta}
	&
	D, \sigma[x \mapsto v_2] \vdash e \Rightarrow v
	&
	D,\rho: e_1 \rightsquigarrow e_1'
	&
	D,\rho : e_2 \rightsquigarrow e_2' 
}
$$

$$
\infer[\textsc{XBuiltin}]{
	\langle D, \rho \vdash f \ e_1 \ \dots \ e_n \Rightarrow v \ | \ f \ v_1 \ \dots \ v_n \Rightarrow v, e_i' \Rightarrow v_i \rangle
}{
	D, \rho \vdash e_i \Rightarrow v_i
	&
	D, \rho : e_i \rightsquigarrow e_i'
	&
	\llbracket f\rrbracket(v_1, \dots, v_n) = v
}
$$

$$
\infer[\textsc{XIfTrue}]{
	\langle D, \rho \vdash \textsf{if } e_1 \ \textsf{then } e_2 \ \textsf{else } e_3 \Rightarrow v \ | \ e_1' \Rightarrow \textsf{True}, e_2' \Rightarrow v \rangle
}{
	D, \rho \vdash e_1 \Rightarrow \textsf{True}
	&
	D, \rho \vdash e_2 \Rightarrow v
	&
	D, \rho : e_1 \rightsquigarrow e_1'
	&
	D, \rho : e_2 \rightsquigarrow e_2'
}
$$

$$
\infer[\textsc{XIfFalse}]{
	\langle D, \rho \vdash \textsf{if } e_1 \ \textsf{then } e_2 \ \textsf{else } e_3 \Rightarrow v \ | \ e_1' \Rightarrow \textsf{False}, e_3' \Rightarrow v \rangle
}{
	D, \rho \vdash e_1 \Rightarrow \textsf{False}
	&
	D, \rho \vdash e_3 \Rightarrow v
	&
	D, \rho : e_1 \rightsquigarrow e_1'
	&
	D, \rho : e_3 \rightsquigarrow e_3'
}
$$
\caption{Operational Semantics for LANG in Explanation Form}
\end{figure*}

\pagebreak

\section*{Explanatory Form for Expressions}

The judgment $\xnf \rho e e'$ means that $e$, in the context of $D$ and $\rho$, has the explanatory form $e'$.



\begin{figure*}[h]

$$
\infer[\textsc{EFVal}]{
    D, \rho : x \rightsquigarrow v
}{
    (x, v) \in \rho
    &
    v \neq (\textsf{closure } y \to e)
}
$$

$$
\infer[\textsc{EFName}]{
    D, \rho : x \rightsquigarrow x
}{}
$$

$$
\infer[\textsc{EFOp}]{
    D, \rho : e_1 \binop e_2 \rightsquigarrow e_1' \binop e_2'
}{
    D, \rho : e_1 \rightsquigarrow e_1'
    &
    D, \rho : e_2 \rightsquigarrow e_2'
}
$$


$$
\infer[\textsc{EFLam}]{
    D, \rho : \codesf{fun } x \ \code{->}\  e \rightsquigarrow \codesf{fun } x \ \code{->}\ e'
}{
    D, \sigma : e \rightsquigarrow e'
    &
    \sigma = \rho \backslash x
}
$$

$$
\infer[\textsc{EFApp}]{
    D, \rho : e_1 \ e_2 \rightsquigarrow e_1' \ e_2'
}{
    D, \rho : e_1 \rightsquigarrow e_1'
    &
    D, \rho : e_2 \rightsquigarrow e_2'
}
$$

$$
\infer[\textsc{EFLet}]{
    D, \rho : \codesf{let } x = e_1 \codesf{ in } e_2 \rightsquigarrow \codesf{let } x = e_1' \codesf{ in } e_2
}{
    \xnf{\rho}{e_1}{e_1'}
    &
    \xnf{\rho}{e_2}{e_2'}
}
$$

$$
\infer[\textsc{EFIf}]{
	D, \rho : \codesf{if}\ e_1\ \codesf{then}\ e_2\ \codesf{else}\ e_3 \rightsquigarrow \codesf{if}\ e_1'\ \codesf{then}\ e_2'\ \codesf{else}\ e_3'
}{
	D, \rho : e_1 \rightsquigarrow e_1'
	&
	D, \rho : e_2 \rightsquigarrow e_2'
	&
	D, \rho : e_3 \rightsquigarrow e_3'
}
$$

$$
\infer[\textsc{EFList}]{
    D, \rho : \codesf [e_1,\ldots,e_n\codesf ] \rightsquigarrow \codesf [e_1',\ldots,e_n'\codesf ]
}{
    D, \rho : e_i \rightsquigarrow e_i'
}
$$	

\caption{Rules for the Explainitory Form for expressions}
\end{figure*}

\pagebreak


%
%\section*{Operational Semantics OLD!}
%
%\begin{gather*}
%\infer[]{\rho : f \ e \rt v}{\rho : e \rt \lambda x.e' & \rho : e \rt v' & \rho[ x\mapsto v' ]: e'\rt v}
%\end{gather*}
%
%\section*{XL Operational Semantics}
%\begin{gather*}
%\infer[]{\textbf X\{ e_1 \ (e_2 \ e_3)\rt v \por e_1 \ v' \rt v\}}{\textbf P\{e_1 \rt \lambda x . e'\} & e_2 \ e_3 \rt v' & [v'/x]e'\rt v}	
%\end{gather*}
%
%\begin{gather*}
%\infer[]{\textbf X\{\code{let $x$ = $e_1$ in $e_2$}\rt v \ | \ e_2\rt v\}}{\textbf P\{e_1 \rt v'\} & v'=\lambda z.e & \textbf P\{[v'/x]e_2\rt v\}}
%\end{gather*}
%
%\begin{gather*}
%\infer[]{\textbf X\{\code{let $x$ = $e_1$ in $e_2$}\rt v \ | \ e_2\rt v\}}{e_1 \rt v'& \textbf P\{[v'/x]e_2\rt v\}}
%\end{gather*}
%
%
%\section*{Post Tagging}
%\begin{gather*}
%\infer[]{}{if condition example }	
%\end{gather*}
%
%\begin{gather*}
%\infer[]{}{e_1\rt \code{True},\code{if $e_1'$ then $e_2'$ else $e_3'$} \rt v_1\vdash \code{if $e_1$ then $e_2$ else $e_3$} \rt v & }	
%\end{gather*}
%
%
%
%
%\pagebreak
%
%\begin{center}
%\begin{tabular}{c}
%$\dfrac{}{D,\rho \vdash v \Rightarrow v}$ \textbf{(Lit)} \\
%\\
%$\dfrac{(x,v) \in \rho}{D,\rho \vdash x \Rightarrow v}$ \textbf{(LocalVar)} \\
%\\
%$\dfrac{(x,e) \in D \qquad D,\{\} \vdash e \Rightarrow v}{D,\rho \vdash x \Rightarrow v}$ \textbf{(GlobalVar)} \\
%\\
%$\dfrac{D,\rho \vdash e_1 \Rightarrow v_1 \qquad D,\rho \vdash e_2 \Rightarrow v_2 \qquad \llbracket op\rrbracket(v_1,v_2) = v}{D,\rho \vdash e_1\ op\ e_2 \Rightarrow v}$ \textbf{(Op)} \\
%\\
%$\dfrac{}{D,\rho \vdash \code{fun } x\code{ -> } e \Rightarrow (\code{closure}\ x\to e,\rho)}$ \textbf{(Abs)} \\
%\\
%$\dfrac{D,\rho \vdash e_1 \Rightarrow (\code{closure}\ x\to e',\rho') \qquad D,\rho \vdash e_2 \Rightarrow v_2 \qquad D,\rho'[x\mapsto v_2] \vdash e' \Rightarrow v}{D,\rho \vdash e_1\ e_2 \Rightarrow v}$ \textbf{(App)} \\
%\\
%$\dfrac{D,\rho \vdash e_1 \Rightarrow v' \qquad D,\rho[x\mapsto v'] \vdash e_2 \Rightarrow v}{D,\rho \vdash \code{let}\ x=e_1\ \code{in}\ e_2 \Rightarrow v}$ \textbf{(Let)} \\
%\\
%$\dfrac{D,\rho \vdash e_1 \Rightarrow \code{True} \qquad D,\rho \vdash e_2 \Rightarrow v_1}{D,\rho \vdash \code{if}\ e_1\ \code{then}\ e_2\ \code{else}\ e_3 \Rightarrow v_1}$ \textbf{(IfTrue)} \\
%\\
%$\dfrac{D,\rho \vdash e_1 \Rightarrow \code{False} \qquad D,\rho \vdash e_3 \Rightarrow v_2}{D,\rho \vdash \code{if}\ e_1\ \code{then}\ e_2\ \code{else}\ e_3 \Rightarrow v_2}$ \textbf{(IfFalse)}
%\end{tabular}
%\end{center}
%
%\pagebreak
%\begin{gather*}
%\infer{\langle D, \rho \vdash v \Rightarrow v \ | \ [] \rangle}{\textsf{XLit}}
%\\\\
%\infer{\langle D, \rho  \vdash x \Rightarrow v \ | \ [] \rangle}{\textsf{XVar}}
%\\\\
%\infer{\langle D, \rho \vdash e_1 + e_2 \Rightarrow v \ | \ e_1' + e_2' \Rightarrow v\rangle}{ D, \rho  \vdash e_1 \Rightarrow v_1 \quad e_1 \rightsquigarrow e_1' \quad  D, \rho \vdash e_2 \Rightarrow v_2 \quad e_2 \rightsquigarrow e_2' \quad v_1 + v_2 = v}{\textsf{XAdd}}
%\\\\
%\infer{\langle D, \rho \vdash \textsf{let } x = e_1 \textsf{ in } e_2 \Rightarrow v \ | \ e_1' \Rightarrow v_1, e_2' \Rightarrow v\rangle}{ D, \rho  \vdash e_1 \Rightarrow v_1 \quad e_1 \rightsquigarrow e_1' \quad D, \rho[x \mapsto v_1]  \vdash e_2 \Rightarrow v \quad e_2 \rightsquigarrow e_2'}{\textsf{XLet}}
%\\\\
%\infer{\langle D, \rho \vdash \textsf{let } x = e_1 \textsf{ in } e_2 \Rightarrow v \ | \ e_2' \Rightarrow v\rangle}{ D, \rho  \vdash e_1 \Rightarrow v_1 \quad v_1= (\textsf{closure} \ z \to e',\rho') \quad D, \rho[x \mapsto v_1]  \vdash e_2 \Rightarrow v \quad e_2 \rightsquigarrow e_2'}{\textsf{XLetFun}}
%\end{gather*}
%$$
%\infer[\textsc{XApp}]{
%	\langle D, \rho \vdash e_1 \ e_2 \Rightarrow v \ | \ e_1' \ v_2 \Rightarrow v, e_2' \Rightarrow v_2, \Delta\rangle
%}{
%	D, \rho  \vdash e_1 \Rightarrow v_1
%	&
%	(\textsf{closure} \ x \to e',\rho' ) = v_1
%	&
%	D, \rho'[x \mapsto v_2] \vdash e' \Rightarrow v
%	&
%	\langle D, \rho \vdash e_2 \Rightarrow v_2 \ | \ \Delta\rangle
%	&
%	D,\rho: e_1 \rightsquigarrow e_1'
%	&
%	D,\rho : e_2 \rightsquigarrow e_2' 
%}
%$$



\end{document}






